compilation.v
@@ -32,6 +32,98 @@ Functional Scheme traduction_ind := Induction for traduction Sort Prop.
 Definition ne_stack (s : stack lambda_term) :=
   exists (e : stack_element lambda_term), exists (tl : stack lambda_term), s = e :: tl.
 
+(**** New version of the soundness ****)
+
+Lemma correction : forall (ti tf : lambda_term), (innermost_strategy ti tf) ->
+  forall (ci cf : code lambda_term) (si : stack lambda_term), ne_stack si -> (well_formed ti) ->
+  ci = traduction ti -> cf = traduction tf -> exists sf : stack lambda_term,
+    ne_stack sf /\
+    cam_reduction_ref_trans lambda_term si (traduction ti) sf nil /\
+    cam_reduction_ref_trans lambda_term si (traduction tf) sf nil.
+Proof.
+  do 3 intro.
+  elim H.
+
+  (* Case of λ *)
+
+  intros.
+  simpl.
+  elim H0; intros.
+  elim H4; clear H4; intros.
+  exists ((avec_code lambda_term (traduction t) x0)::x1).
+  split.
+  unfold ne_stack.
+  exists (avec_code lambda_term (traduction t) x0).
+  exists x1; auto.
+  rewrite H4.
+  split; simplification_cam.
+
+  (* Case of application *)
+
+	intros.
+	simpl.
+	elim H8; intros; elim H12; intros; rewrite H13.
+  elim (well_formed_app _ _ H9); intros.
+	assert (well_formed t4). apply redex_well_formed with (lapp t1' t2'). apply application_wf. apply  innermost_strategy_well_formed with t1. apply H14. apply H0. apply innermost_strategy_well_formed with t2. apply H15. apply H2. apply Beta_redex_ref_trans. apply H5.
+	elim (H1 (traduction t1) (traduction t1') (x0::x0::x1)); clear H1; intros; auto;
+	  [idtac | unfold ne_stack; exists x0; exists (x0 :: x1); auto].
+	elim H1; clear H1; intros.
+	elim H1; clear H1; intros.
+	elim H17; clear H17; intros.
+	clear H9 H12.
+	rewrite H4 in H18.
+	simpl in H18.
+	elim (stack_two lambda_term x0 x0 x1 x2 (traduction t3) nil H18); intros.
+	elim H9; clear H9; intros.
+	elim H9; clear H9; intros.
+	rewrite 
+	elim (H3 (traduction t2) (traduction t2') (x5::x4::x6)); clear H3; intros; auto;
+	  [idtac | unfold ne_stack; exists x5; exists (x4::x6); auto].
+	elim H3; clear H3; intros.
+	elim H3; clear H3; intros.
+	elim H12; clear H12; intros.
+  rewrite H4 in H5.
+  elim (beta_cam t3 t2' t4 si H8 H5); intros.
+  elim H20; clear H20; intros.
+  elim H20; clear H20; intros.
+  elim H21; clear H21; intros.
+  simpl in H21.
+  elim (H7 (traduction t4) (traduction t4') si H8 H16); clear H7; intros; auto.
+  elim H7; clear H7; intros.
+  elim H7; clear H7; intros.
+  elim H23; clear H23; intros.
+  exists x11.
+  exists x12.
+  rewrite H13 in H23, H24.
+  split; auto.
+  split; auto.
+  cut (cam_reduction_ref_trans lambda_term si
+    (pushl :: traduction t1 ++ swapl :: traduction t2 ++ appl :: nil) x9 x10).
+  intro.
+  generalize (equality _ _ _ _ _ H8 H22 H25); intro.
+  rewrite <- H26; assumption.
+  rewrite H13.
+  simplification_cam.
+  apply reduc_trans with x2 (x3 ++ swapl :: traduction t2 ++ appl :: nil).
+  Focus 2.
+  rewrite H9.
+
+
+
+
+
+(**** Old version of the soundness ***)
+
+Axiom beta_cam : forall (t u t' : lambda_term) (si : stack lambda_term), ne_stack si ->
+  (lapp (λ t) u) ->β t' -> 
+  exists sf : stack lambda_term, exists c : code lambda_term,
+    ne_stack sf /\
+    cam_reduction_ref_trans lambda_term si (traduction (lapp (λ t) u)) sf c /\
+    cam_reduction_ref_trans lambda_term si (traduction t') sf c.
+
+Axiom equality : forall (si sf : stack lambda_term) (c c' cf : code lambda_term), ne_stack si ->
+  cam_reduction_ref_trans lambda_term si c sf cf -> cam_reduction_ref_trans lambda_term si c' sf cf -> c = c'.
+
 Lemma correction : forall (ti tf : lambda_term), (innermost_strategy ti tf) ->
   forall (ci cf : code lambda_term) (si : stack lambda_term), ne_stack si -> (well_formed ti) ->
   ci = traduction ti -> cf = traduction tf -> exists sf : stack lambda_term, exists c : code lambda_term,
@@ -90,8 +182,83 @@ Proof.
 	simpl.
 	elim H8; intros; elim H12; intros; rewrite H13.
 	elim (well_formed_app _ _ H9); intros.
-	assert (well_formed t4). apply redex_well_formed with (lapp t1' t2'). apply application_wf. apply  innermost_strategy_well_formed with t1. apply H14. apply H0. apply innermost_strategy_well_formed with t2. apply H15. apply H2. apply Beta_redex_ref_trans. apply H5. 
-	elim (H7 (traduction t4) (traduction t4') (x0 :: x1)); intros; auto; [ idtac | unfold ne_stack; exists x0; exists x1; auto ].
-	elim H17; clear H17; intros; inversion_clear H17; inversion_clear H19.
-²
-	
+	assert (well_formed t4). apply redex_well_formed with (lapp t1' t2'). apply application_wf. apply  innermost_strategy_well_formed with t1. apply H14. apply H0. apply innermost_strategy_well_formed with t2. apply H15. apply H2. apply Beta_redex_ref_trans. apply H5.
+	elim (H1 (traduction t1) (traduction t1') (x0::x0::x1)); clear H1; intros; auto;
+	  [idtac | unfold ne_stack; exists x0; exists (x0 :: x1); auto].
+	elim H1; clear H1; intros.
+	elim H1; clear H1; intros.
+	elim H17; clear H17; intros.
+	clear H9 H12.
+	rewrite H4 in H18.
+	simpl in H18.
+	elim (stack_two lambda_term x0 x0 x1 x2 (traduction t3) nil x3 H18); intros.
+	elim H9; clear H9; intros.
+	elim H9; clear H9; intros.
+	elim (H3 (traduction t2) (traduction t2') (x5::x4::x6)); clear H3; intros; auto;
+	  [idtac | unfold ne_stack; exists x5; exists (x4::x6); auto].
+	elim H3; clear H3; intros.
+	elim H3; clear H3; intros.
+	elim H12; clear H12; intros.
+  rewrite H4 in H5.
+  elim (beta_cam t3 t2' t4 si H8 H5); intros.
+  elim H20; clear H20; intros.
+  elim H20; clear H20; intros.
+  elim H21; clear H21; intros.
+  simpl in H21.
+  elim (H7 (traduction t4) (traduction t4') si H8 H16); clear H7; intros; auto.
+  elim H7; clear H7; intros.
+  elim H7; clear H7; intros.
+  elim H23; clear H23; intros.
+  exists x11.
+  exists x12.
+  rewrite H13 in H23, H24.
+  split; auto.
+  split; auto.
+  cut (cam_reduction_ref_trans lambda_term si
+    (pushl :: traduction t1 ++ swapl :: traduction t2 ++ appl :: nil) x9 x10).
+  intro.
+  generalize (equality _ _ _ _ _ H8 H22 H25); intro.
+  rewrite <- H26; assumption.
+  rewrite H13.
+  simplification_cam.
+  apply reduc_trans with x2 (x3 ++ swapl :: traduction t2 ++ appl :: nil).
+  Focus 2.
+  rewrite H9.
+  
+
+
+
+
+
+
+
+
+
+
+
+
+
+
+
+
+
+
+
+
+
+
+
+
+
+
+
+
+
+
+
+
+
+
+
+
+
